ContainersPlugin/theories/OrderedType.v
@@ -423,30 +423,6 @@ Ltac order :=
 Ltac false_order := elimtype False; order.
 
 (*
-Instance Proper_eq_fun (X:Type) H0 (f:X->X)
-:  @Proper (X -> X)
-           (@respectful X X
-                        (@_eq X (@SOT_as_OT X (@eq X) H0))
-                        (@_eq X (@SOT_as_OT X (@eq X) H0))) f.
-Proof.
-  intuition.
-Qed.
-
--Hint Extern 5 (_eq _ _) => reflexivity.
--Hint Extern 5 (_ === _) => reflexivity.
--Hint Extern 10 (_eq _ _) => symmetry; assumption.
--Hint Extern 10 (_ === _) => symmetry; assumption.
--Hint Extern 11 (Equivalence _) => constructor; congruence.
--Hint Extern 11 (Equivalence _) => apply OT_Equivalence.
--Hint Extern 11 (StrictOrder _) => apply OT_StrictOrder.
--Hint Extern 11 (RelationClasses.StrictOrder _) =>
--constructor; repeat intro; order.
--(*Hint Extern 1 (Proper _ _) => eassumption.
--Hint Extern 8 (Proper _ _) => apply lt_m. *)
--Hint Extern 9 (Proper _ _) =>
--first [ eassumption | apply lt_m | apply Proper_eq_fun | repeat intro; intuition order ].
-*)
-
 Hint Extern 0 (_eq _ _) => reflexivity.
 Hint Extern 0 (_ === _) => reflexivity.
 Hint Extern 2 (_eq _ _) => symmetry; assumption.
@@ -458,6 +434,7 @@ Hint Extern 1 (RelationClasses.StrictOrder _) =>
   constructor; repeat intro; order.
 Hint Extern 1 (Proper _ _) => apply lt_m.
 Hint Extern 1 (Proper _ _) => repeat intro; intuition order.
+ *)
 
 (** ** Specific Ordered types : [OrderedType] with specific equality
 
@@ -468,6 +445,7 @@ Hint Extern 1 (Proper _ _) => repeat intro; intuition order.
    also match [OrderedType]. An alternative would be to take the equality
    relation ouf of the [OrderedType] instance and add it as a parameter.
 *)
+
 Class SpecificOrderedType
   (A : Type) (eqA : relation A) := {
   SOT_Equivalence :> Equivalence eqA ;
@@ -494,6 +472,27 @@ Defined.
    *)
 Notation "'UsualOrderedType' A" :=
   (SpecificOrderedType A (@eq A))(at level 30).
+
+Instance Proper_eq_fun (X:Type) (H0:UsualOrderedType X) (f:X->X)
+:  @Proper (X -> X)
+           (@respectful X X
+                        (@_eq X (@SOT_as_OT X (@eq X) H0))
+                        (@_eq X (@SOT_as_OT X (@eq X) H0))) f.
+Proof.
+  intuition.
+Qed.
+
+Hint Extern 5 (_eq _ _) => reflexivity.
+Hint Extern 5 (_ === _) => reflexivity.
+Hint Extern 10 (_eq _ _) => symmetry; assumption.
+Hint Extern 10 (_ === _) => symmetry; assumption.
+Hint Extern 11 (Equivalence _) => constructor; congruence.
+Hint Extern 11 (Equivalence _) => apply OT_Equivalence.
+Hint Extern 11 (StrictOrder _) => apply OT_StrictOrder.
+Hint Extern 11 (RelationClasses.StrictOrder _) =>
+constructor; repeat intro; order.
+Hint Extern 9 (Proper _ _) =>
+first [ eassumption | apply lt_m | apply Proper_eq_fun | repeat intro; intuition order ].
 
 (** * Facts about setoid list membership
 
