theories/Infra/Status.v
@@ -188,6 +188,8 @@ Inductive status_eq {A} (eqA : relation A) : status A -> status A -> Prop :=
 | status_eq_Error s : status_eq eqA (Error s) (Error s)
 | status_eq_Some : forall a a', eqA a a' -> status_eq eqA (Success a) (Success a').
 
+Require Import Containers.Tactics.
+
 Program Instance success_Equivalence A eqA `(Equivalence A eqA) :
   Equivalence (status_eq eqA).
 Next Obligation. (* reflexivity *)
